concurrency/sync_preds.v
@@ -314,12 +314,12 @@ Qed.
 
 Lemma jstep_preserves_mem_equiv_on_other_threads m ge i j tp ci ci' jmi'
   (other : i <> j)
-  (compat : mem_compatible tp m)
+  compat
   cnti cntj
   (tp' := age_tp_to (level (m_phi jmi')) tp)
   (tp'' := @updThread i tp' (cnt_age' cnti) (Krun ci') (m_phi jmi') : thread_pool)
   (stepi : @jstep genv corestate cl_core_sem ge ci (@personal_mem i tp m cnti compat) ci' jmi')
-  (compat': mem_compatible tp'' (m_dry jmi')) :
+  compat' :
   mem_equiv
     (m_dry (@personal_mem j tp m cntj compat))
     (m_dry (@personal_mem j tp'' (m_dry jmi') (cnt_age' cntj) compat')).
